Change how TraceSegment splitting is done
Previously, the argument 'k' given to indicate the split location was
relative to the full trace. With this change, it is relative to the
beginning of the segment instead. As a result, we no longer have to
reference seg.i and seg.j (the starting and ending locations of the
trace, which are intended to be private) and can instead reference only
the segment length.

AngelDevil/Segment.lean
@@ -63,23 +63,23 @@ def segment_states (seg : TraceSegment) : List RunState :=
 def segment_length (seg : TraceSegment) : Nat := seg.j - seg.i + 1
 
 -- Split the segment into two pieces and take the first part
-def segment_split_first (seg : TraceSegment) (k : Nat) (lek : seg.i ≤ k) (kle : k ≤ seg.j) : TraceSegment where
+def segment_split_first (seg : TraceSegment) (k : Nat) (klt : k < segment_length seg) : TraceSegment where
   n := seg.n
   start := seg.start
   blocked := seg.blocked
   i := seg.i
-  j := k
-  ile := lek
-  jlt := lt_of_le_of_lt kle seg.jlt
+  j := seg.i + k
+  ile := Nat.le_add_right _ _
+  jlt := lt_of_le_of_lt (Nat.add_le_of_le_sub' seg.ile (Nat.le_of_lt_add_one klt)) seg.jlt
 
 -- Split the segment into two pieces and take the second part
-def segment_split_second (seg : TraceSegment) (k : Nat) (_ : seg.i ≤ k) (kle : k ≤ seg.j) : TraceSegment where
+def segment_split_second (seg : TraceSegment) (k : Nat) (klt : k < segment_length seg) : TraceSegment where
   n := seg.n
   start := seg.start
   blocked := seg.blocked
-  i := k
+  i := seg.i + k
   j := seg.j
-  ile := kle
+  ile := Nat.add_le_of_le_sub' seg.ile (Nat.le_of_lt_add_one klt)
   jlt := seg.jlt
 
 lemma segment_length_pos (seg : TraceSegment) :
@@ -116,111 +116,100 @@ lemma segment_end_eq_getElem (seg : TraceSegment) :
   apply (Nat.add_sub_cancel' _).symm
   exact seg.ile
 
-lemma segment_split_first_start (seg : TraceSegment) (k : Nat) (lek : seg.i ≤ k) (kle : k ≤ seg.j) :
-  segment_start (segment_split_first seg k lek kle) = segment_start seg := rfl
+lemma segment_split_first_start (seg : TraceSegment) (k : Nat) (klt : k < segment_length seg) :
+  segment_start (segment_split_first seg k klt) = segment_start seg := rfl
 
-lemma segment_split_second_end (seg : TraceSegment) (k : Nat) (lek : seg.i ≤ k) (kle : k ≤ seg.j) :
-  segment_end (segment_split_second seg k lek kle) = segment_end seg := rfl
+lemma segment_split_second_end (seg : TraceSegment) (k : Nat) (klt : k < segment_length seg) :
+  segment_end (segment_split_second seg k klt) = segment_end seg := rfl
 
-lemma segment_split_overlap (seg : TraceSegment) (k : Nat) (lek : seg.i ≤ k) (kle : k ≤ seg.j) :
-  segment_end (segment_split_first seg k lek kle) =
-  segment_start (segment_split_second seg k lek kle) := rfl
+lemma segment_split_overlap (seg : TraceSegment) (k : Nat) (klt : k < segment_length seg) :
+  segment_end (segment_split_first seg k klt) =
+  segment_start (segment_split_second seg k klt) := rfl
 
 -- Get the length of the first half of a split trace
-lemma segment_split_first_length (seg : TraceSegment) (k : Nat) (lek : seg.i ≤ k) (kle : k ≤ seg.j) :
-  segment_length (segment_split_first seg k lek kle) = k - seg.i + 1 := by
+lemma segment_split_first_length (seg : TraceSegment) (k : Nat) (klt : k < segment_length seg) :
+  segment_length (segment_split_first seg k klt) = k + 1 := by
   unfold segment_length segment_split_first; simp
 
 -- Get the length of the second half of a split trace
-lemma segment_split_second_length (seg : TraceSegment) (k : Nat) (lek : seg.i ≤ k) (kle : k ≤ seg.j) :
-  segment_length (segment_split_second seg k lek kle) = seg.j - k + 1 := by
+lemma segment_split_second_length (seg : TraceSegment) (k : Nat) (klt : k < segment_length seg) :
+  segment_length (segment_split_second seg k klt) = segment_length seg - k := by
   unfold segment_length segment_split_second; simp
+  rw [Nat.sub_add_eq, Nat.sub_add_comm]
+  exact Nat.le_of_lt_add_one klt
 
 -- The length of a segment is one less than the sum of the
 -- lengths of its two parts
-lemma segment_split_length (seg : TraceSegment) (k : Nat) (lek : seg.i ≤ k) (kle : k ≤ seg.j) :
+lemma segment_split_length (seg : TraceSegment) (k : Nat) (klt : k < segment_length seg) :
   segment_length seg =
-  (segment_length (segment_split_first seg k lek kle)) +
-  (segment_length (segment_split_second seg k lek kle)) - 1 := by
-  rw [segment_split_first_length, segment_split_second_length, segment_length]; simp
-  rw [add_comm _ (seg.j - k), ← add_assoc, ← Nat.add_sub_assoc lek]
-  rw [Nat.sub_add_cancel kle]
+  (segment_length (segment_split_first seg k klt)) +
+  (segment_length (segment_split_second seg k klt)) - 1 := by
+  rw [segment_split_first_length, segment_split_second_length]; simp
+  exact (Nat.add_sub_cancel' (le_of_lt klt)).symm
 
 -- Get an element from the first half of a split trace segment
 lemma segment_split_first_states_getElem
-  (seg : TraceSegment) (k : Nat) (lek : seg.i ≤ k) (kle : k ≤ seg.j) :
-  ∀ a (alt : a < (segment_states (segment_split_first seg k lek kle)).length),
-  (segment_states (segment_split_first seg k lek kle))[a] =
+  (seg : TraceSegment) (k : Nat) (klt : k < segment_length seg) :
+  ∀ a (alt : a < (segment_states (segment_split_first seg k klt)).length),
+  (segment_states (segment_split_first seg k klt))[a] =
   (segment_states seg)[a]'(by
     rw [segment_states_length, segment_split_first_length] at alt
-    rw [segment_states_length, segment_length]
-    exact lt_of_lt_of_le alt ((Nat.add_le_add_right (Nat.sub_le_sub_right kle _)) _)
+    rw [segment_states_length]
+    exact lt_of_le_of_lt (Nat.le_of_lt_add_one alt) klt
   ) := by
   intro _ _
   unfold segment_states segment_split_first segment_trace; simp
 
 -- Get an element from the second half of a split trace segment
 lemma segment_split_second_states_getElem
-  (seg : TraceSegment) (k : Nat) (lek : seg.i ≤ k) (kle : k ≤ seg.j) :
-  ∀ a (alt : a < (segment_states (segment_split_second seg k lek kle)).length),
-  (segment_states (segment_split_second seg k lek kle))[a] =
-  (segment_states seg)[a + k - seg.i]'(by
+  (seg : TraceSegment) (k : Nat) (klt : k < segment_length seg) :
+  ∀ a (alt : a < (segment_states (segment_split_second seg k klt)).length),
+  (segment_states (segment_split_second seg k klt))[a] =
+  (segment_states seg)[a + k]'(by
     rw [segment_states_length, segment_split_second_length] at alt
-    rw [segment_states_length, segment_length]
-    apply Nat.sub_lt_right_of_lt_add (le_trans lek (Nat.le_add_left _ _))
-    rw [add_right_comm, Nat.sub_add_cancel]; swap
-    · exact le_trans lek kle
-    apply Nat.add_lt_of_lt_sub
-    rwa [Nat.sub_add_comm]
-    exact kle
-  ) := by
+    rw [segment_states_length]
+    exact Nat.add_lt_of_lt_sub alt) := by
   intro a alt
   unfold segment_states segment_split_second segment_trace; simp; congr 1
-  rw [add_comm, add_comm seg.i, Nat.sub_add_cancel]
-  exact le_trans lek (Nat.le_add_left _ _)
+  rw [add_comm a, add_assoc]
 
 -- Prove an identity for the states of the first half of a split segment
-lemma segment_split_first_states (seg : TraceSegment) (k : Nat) (lek : seg.i ≤ k) (kle : k ≤ seg.j) :
-  segment_states (segment_split_first seg k lek kle) =
-  List.take (k - seg.i + 1) (segment_states seg) := by
+lemma segment_split_first_states (seg : TraceSegment) (k : Nat) (klt : k < segment_length seg) :
+  segment_states (segment_split_first seg k klt) =
+  List.take (k + 1) (segment_states seg) := by
   apply List.ext_getElem
   · rw [segment_states_length, segment_split_first_length]
     rw [List.length_take_of_le]
-    rw [segment_states_length, segment_length]
-    exact Nat.add_le_add_right (Nat.sub_le_sub_right kle _) _
+    rw [segment_states_length]
+    exact Nat.add_one_le_of_lt klt
   intro a alt alt'
   rw [segment_split_first_states_getElem, List.getElem_take]
 
 -- Prove an identity for the states of the second half of a split segment
-lemma segment_split_second_states (seg : TraceSegment) (k : Nat) (lek : seg.i ≤ k) (kle : k ≤ seg.j) :
-  segment_states (segment_split_second seg k lek kle) =
-  List.drop (k - seg.i) (segment_states seg) := by
+lemma segment_split_second_states (seg : TraceSegment) (k : Nat) (klt : k < segment_length seg) :
+  segment_states (segment_split_second seg k klt) =
+  List.drop k (segment_states seg) := by
   apply List.ext_getElem
   · rw [segment_states_length, segment_split_second_length, List.length_drop]
-    rw [segment_states_length, segment_length]
-    rw [Nat.sub_sub_right _ lek, add_right_comm _ 1]
-    rw [Nat.sub_add_cancel (le_trans lek kle)]
-    rw [Nat.sub_add_comm]
-    exact kle
+    rw [segment_states_length]
   intro a alt _
-  rw [segment_split_second_states_getElem, List.getElem_drop]; congr
-  rw [add_comm (k - seg.i), Nat.add_sub_assoc]
-  exact lek
+  rw [segment_split_second_states_getElem, List.getElem_drop]; congr 1
+  exact add_comm _ _
 
 -- The list of states for a split segment is equal to those
 -- in the first part followed by the tail of those in the second
-lemma segment_split_states (seg : TraceSegment) (k : Nat) (lek : seg.i ≤ k) (kle : k ≤ seg.j) :
+lemma segment_split_states (seg : TraceSegment) (k : Nat) (klt : k < segment_length seg) :
   segment_states seg =
-  segment_states (segment_split_first seg k lek kle) ++
-  (segment_states (segment_split_second seg k lek kle)).tail := by
+  segment_states (segment_split_first seg k klt) ++
+  (segment_states (segment_split_second seg k klt)).tail := by
   apply List.ext_getElem
   · rw [List.length_append, List.length_tail, ← Nat.add_sub_assoc]; swap
-    · rw [segment_states_length]
-      unfold segment_length segment_split_second; simp
+    · rw [segment_states_length, segment_split_second_length]
+      exact Nat.le_sub_of_add_le' (Nat.add_one_le_of_lt klt)
     repeat rw [segment_states_length]
-    exact segment_split_length seg k lek kle
+    exact segment_split_length seg k klt
   intro a alt _
-  by_cases alt' : a < (segment_states (segment_split_first seg k lek kle)).length
+  by_cases alt' : a < (segment_states (segment_split_first seg k klt)).length
   · rw [List.getElem_append_left alt']
     rw [segment_split_first_states_getElem]
   · rename' alt' => lea; push_neg at lea
@@ -228,10 +217,7 @@ lemma segment_split_states (seg : TraceSegment) (k : Nat) (lek : seg.i ≤ k) (k
     rw [segment_split_second_states_getElem]
     congr
     rw [segment_states_length, segment_split_first_length]
-    rw [add_assoc, Nat.add_sub_assoc, add_comm 1]; swap
-    · rw [add_comm]
-      exact le_of_lt (lt_of_le_of_lt lek (Nat.lt_add_one _))
-    rw [Nat.sub_add_comm lek, Nat.sub_add_cancel]
+    rw [add_assoc, Nat.add_comm 1, Nat.sub_add_cancel]
     rwa [segment_states_length, segment_split_first_length] at lea
 
 -- Check if the 'move' between state 'a' and state 'a+1' is 'f'
@@ -254,16 +240,16 @@ def segment_starts_with_turn_right (seg : TraceSegment) (h : 1 < segment_length 
 -- A split segment starts with a particular move if the original segment did
 def segment_split_first_starts_with_move (seg : TraceSegment) (h : 1 < segment_length seg)
   (f : RunState → RunState) (hmove : check_for_move seg f 0 h) :
-  ∀ k (ltk : seg.i < k) (kle : k ≤ seg.j),
-  check_for_move (segment_split_first seg k (le_of_lt ltk) kle) f 0
+  ∀ k (kpos : 0 < k) (klt : k < segment_length seg),
+  check_for_move (segment_split_first seg k klt) f 0
   (by
     rw [segment_split_first_length]
-    exact Nat.add_one_lt_add_one_iff.mpr (Nat.sub_pos_of_lt ltk)
+    exact Nat.add_one_lt_add_one_iff.mpr kpos
   ) := by
-  intro k ltk kle
-  have lek : seg.i ≤ k := le_of_lt ltk
+  intro k kpos klt
+  ---have lek : seg.i ≤ k := le_of_lt ltk
   unfold check_for_move at *
-  repeat rw [getElem_congr_coll (segment_split_first_states seg k lek kle)]
+  repeat rw [getElem_congr_coll (segment_split_first_states seg k klt)]
   rwa [List.getElem_take, List.getElem_take]
 
 -- The segment begins with a left turn and continues straight
@@ -276,13 +262,11 @@ def segment_is_L (seg : TraceSegment) (h : 1 < segment_length seg) : Prop :=
 def segment_is_U (seg : TraceSegment) (h : 2 < segment_length seg) : Prop :=
   (fun segL sllb ↦ segment_is_L segL sllb ∧
   segment_end seg = turn_left (segment_end segL))
-  (segment_split_first seg (seg.j - 1) (by
-    apply Nat.le_sub_one_of_lt (Nat.lt_of_sub_pos _)
-    exact Nat.add_one_lt_add_one_iff.mp (lt_trans (by norm_num) h)) (Nat.sub_le _ _))
+  (segment_split_first seg (segment_length seg - 2)
+    (Nat.sub_lt (Nat.zero_lt_of_lt h) (Nat.two_pos)))
   (by
-    rw [segment_split_first_length, Nat.sub_right_comm]
-    rw [← Nat.sub_add_comm (Nat.add_one_le_add_one_iff.mp (le_of_lt h))]
-    exact Nat.lt_sub_of_add_lt h)
+    rw [segment_split_first_length]
+    exact Nat.add_one_lt_add_one_iff.mpr (Nat.lt_sub_of_add_lt ((Nat.zero_add 2) ▸ h)))
 
 -- Write the end of an 'L' segment in terms of the start
 lemma segment_end_of_L (seg : TraceSegment) (h : 1 < segment_length seg) :
@@ -316,114 +300,73 @@ lemma segment_end_of_L (seg : TraceSegment) (h : 1 < segment_length seg) :
   have sllb : 2 < segment_length seg := by
     apply lt_of_le_of_ne _ hslne2.symm
     exact Nat.add_one_le_of_lt h
-  have iltj : seg.i < seg.j :=
-    Nat.lt_of_sub_pos (Nat.add_one_lt_add_one_iff.mp h)
-  have jpos : 0 < seg.j :=
-    Nat.zero_lt_of_lt iltj
-  let k := seg.j - 1
-  have ltk : seg.i < k := by
-    apply Nat.add_one_lt_add_one_iff.mp
-    rw [Nat.sub_one_add_one (Nat.ne_zero_of_lt jpos), add_comm]
-    apply Nat.add_lt_of_lt_sub
-    exact Nat.add_one_le_add_one_iff.mp sllb
-  have lek : seg.i ≤ k := le_of_lt ltk
-  have kle : k ≤ seg.j :=
-    Nat.sub_le _ _
+  have s2a1 {n : Nat} (onelt : 1 < n) : n - 2 + 1 = n - 1 := by
+    rw [← one_add_one_eq_two, Nat.sub_add_eq]
+    rw [Nat.sub_one_add_one (Nat.sub_ne_zero_of_lt onelt)]
+  let k := segment_length seg - 2
+  have klt : k < segment_length seg :=
+    Nat.sub_lt (Nat.zero_lt_of_lt h) Nat.two_pos
+  have kpos : 0 < k := Nat.sub_pos_of_lt sllb
   -- Split the segment into an L segment, and a single forward step
-  let seg_first := segment_split_first seg k lek kle
+  let seg_first := segment_split_first seg k klt
   have hsflb : 1 < segment_length seg_first := by
     rw [segment_split_first_length]
-    rw [Nat.sub_right_comm, Nat.sub_one_add_one (Nat.sub_ne_zero_of_lt iltj)]
-    exact Nat.add_one_lt_add_one_iff.mp sllb
+    exact Nat.add_one_lt_add_one_iff.mpr kpos
+  have kslt : k + 1 < segment_length seg := by
+    unfold k
+    rw [s2a1 h]
+    exact Nat.sub_lt (Nat.zero_lt_of_lt h) Nat.one_pos
   have hsfL : segment_is_L seg_first hsflb := by
     constructor
-    · exact segment_split_first_starts_with_move seg h turn_left hL k ltk kle
+    · exact segment_split_first_starts_with_move seg h turn_left hL k kpos klt
     · intro a aslt anz
       unfold check_for_move
-      repeat rw [getElem_congr_coll (segment_split_first_states seg k lek kle)]
+      repeat rw [getElem_congr_coll (segment_split_first_states seg k klt)]
       rw [List.getElem_take, List.getElem_take]
       apply hMF a _ anz
       apply lt_trans aslt
-      rw [segment_split_first_length, segment_length]
-      rw [Nat.sub_right_comm]
-      apply Nat.add_one_lt_add_one_iff.mpr
-      exact Nat.sub_one_lt (Nat.sub_ne_zero_of_lt iltj)
+      rwa [segment_split_first_length]
   -- Recursively write the end of 'first_seg' in terms of 'segment_start'
   have hend₀ := segment_end_of_L seg_first hsflb hsfL
   -- Write the end of the segment in terms of the end of 'first_seg'
   have hend₁ : segment_end seg = move_forward (segment_end seg_first) := by
     rw [segment_end_eq_getElem, segment_end_eq_getElem]
     rw [segment_split_first_states_getElem]
-    have sfl := congrArg (fun n ↦ n - 1) (segment_split_first_length seg k lek kle); simp at sfl
-    rw [getElem_congr_idx sfl]
-    unfold segment_length
-    rw [getElem_congr_idx (Nat.add_one_sub_one _)]
-    have s2a1 (n : Nat) (onelt : 1 < n) : n - 2 + 1 = n - 1 := by
-      rw [← one_add_one_eq_two, Nat.sub_add_eq]
-      rw [Nat.sub_one_add_one]
-      exact Nat.sub_ne_zero_of_lt onelt
-    have hlt : segment_length seg - 2 + 1 < segment_length seg := by
-      rw [s2a1 _ h]
-      exact Nat.sub_one_lt (Nat.ne_zero_of_lt h)
-    have := hMF (segment_length seg - 2) hlt (Nat.sub_ne_zero_of_lt sllb)
-    unfold check_for_move at this
+    have := hMF k kslt (Nat.ne_zero_of_lt kpos)
     convert this.symm using 2
-    · unfold segment_length
-      rw [s2a1, Nat.add_one_sub_one]
-      apply Nat.add_one_lt_add_one_iff.mpr
-      exact Nat.sub_pos_of_lt iltj
+    · exact Nat.eq_add_of_sub_eq (Nat.le_sub_one_of_lt h) rfl
     · congr 1
-      unfold segment_length k
-      rw [Nat.sub_right_comm]
-      apply Nat.add_one_inj.mp
-      rw [Nat.sub_one_add_one (Nat.sub_ne_zero_of_lt iltj)]
-      rw [s2a1, Nat.add_one_sub_one]
-      apply Nat.add_one_lt_add_one_iff.mpr
-      exact Nat.sub_pos_of_lt iltj
+      rw [segment_split_first_length]; simp
   rw [hend₁, hend₀, segment_split_first_start, segment_split_first_length]
   unfold move_forward rotate_left k
-  apply RunState.ext
-  · simp
-    rw [add_right_comm _ (segment_start seg).x]
+  apply RunState.ext <;> simp
+  · rw [add_right_comm _ (segment_start seg).x]
     apply (Int.add_left_inj _).mpr
     rw [add_right_comm]
     apply (Int.add_left_inj _).mpr
     rw [← Int.neg_add]
     nth_rw 2 [← one_mul (segment_start seg).u.y]
     rw [← Int.add_mul]; congr
-    rw [Nat.sub_right_comm]
-    rw [← Nat.add_one_sub_one (seg.j - seg.i)]
-    rw [Int.ofNat_sub]; swap
-    · rw [Nat.add_one_sub_one]
-      apply Nat.add_one_le_of_lt
-      exact Nat.sub_pos_of_lt iltj
-    rw [Int.ofNat_sub]; swap
-    · exact Nat.add_one_le_add_one_iff.mpr (Nat.zero_le _)
-    rw [Int.ofNat_one, Int.sub_add_cancel]
-    rfl
-  · simp
-    rw [add_right_comm _ (segment_start seg).y]
+    rw [← Int.natCast_one, ← Int.natCast_add]
+    rw [s2a1 h, Int.natCast_sub]
+    exact le_of_lt h
+  · rw [add_right_comm _ (segment_start seg).y]
     apply (Int.add_left_inj _).mpr
     rw [add_right_comm]
     apply (Int.add_left_inj _).mpr
     nth_rw 2 [← one_mul (segment_start seg).u.x]
     rw [← Int.add_mul]; congr
-    rw [Nat.sub_right_comm]
-    rw [← Nat.add_one_sub_one (seg.j - seg.i)]
-    rw [Int.ofNat_sub]; swap
-    · rw [Nat.add_one_sub_one]
-      apply Nat.add_one_le_of_lt
-      exact Nat.sub_pos_of_lt iltj
-    rw [Int.ofNat_sub]; swap
-    · exact Nat.add_one_le_add_one_iff.mpr (Nat.zero_le _)
-    rw [Int.ofNat_one, Int.sub_add_cancel]
-    rfl
-  · simp
+    rw [← Int.natCast_one, ← Int.natCast_add]
+    rw [s2a1 h, Int.natCast_sub]
+    exact le_of_lt h
 termination_by (segment_length seg)
 decreasing_by
-  rw [segment_split_first_length, Nat.sub_right_comm]
-  rw [Nat.sub_one_add_one (Nat.sub_ne_zero_of_lt iltj)]
-  exact Nat.lt_add_one _
+  -- For some reason Lean isn't giving us the right context here
+  -- so we can't use 's2a1'. Just copy and paste the logic from there.
+  rw [segment_split_first_length]
+  rw [← one_add_one_eq_two, Nat.sub_add_eq]
+  rw [Nat.sub_one_add_one (Nat.sub_ne_zero_of_lt h)]
+  exact Nat.sub_lt (Nat.zero_lt_of_lt h) Nat.one_pos
 
 -- Write the end of a 'U' segment in terms of the start
 lemma segment_end_of_U (seg : TraceSegment) (h : 2 < segment_length seg) :
@@ -435,41 +378,33 @@ lemma segment_end_of_U (seg : TraceSegment) (h : 2 < segment_length seg) :
   ) (segment_start seg) (segment_length seg - 1) := by
   unfold segment_is_U
   intro ⟨hL, hlast⟩
-  let k := seg.j - 1
-  have ltk : seg.i < k := by
-    apply Nat.lt_sub_of_add_lt
-    rw [add_comm]
-    exact Nat.add_lt_of_lt_sub (Nat.add_one_lt_add_one_iff.mp h)
-  have lek := le_of_lt ltk
-  have kle : k ≤ seg.j := Nat.sub_le _ _
-  let seg_first := segment_split_first seg (seg.j - 1) lek kle
+  let k := segment_length seg - 2
+  have klt : k < segment_length seg :=
+    Nat.sub_lt (Nat.zero_lt_of_lt h) Nat.two_pos
+  have kpos : 0 < k := Nat.sub_pos_of_lt h
+  have ks : k + 1 = segment_length seg - 1 := by
+    unfold k
+    rw [← one_add_one_eq_two, Nat.sub_add_eq, Nat.sub_one_add_one]
+    exact Nat.sub_ne_zero_of_lt (lt_trans (by norm_num) h)
+  let seg_first := segment_split_first seg k klt
   have slssf : 1 < segment_length seg_first := by
     rw [segment_split_first_length]
-    exact Nat.add_one_lt_add_one_iff.mpr (Nat.sub_pos_of_lt ltk)
+    exact Nat.add_one_lt_add_one_iff.mpr kpos
+  have lesl : 1 ≤ segment_length seg := le_of_lt (lt_trans (by norm_num) h)
   rw [hlast, segment_end_of_L _ slssf hL, segment_split_first_start]
   rw [segment_split_first_length]
   unfold turn_left rotate_left
-  -- Miscellaneous bounds checks we'll need below
-  have hle₀ := Nat.add_one_le_add_one_iff.mp (le_of_lt h)
-  have hle₁ : 1 ≤ seg.j - seg.i + 1 :=
-    le_of_lt (lt_trans (by norm_num) h)
   apply RunState.ext <;> simp
   · rw [add_right_comm, add_right_comm _ _ (-(segment_start seg).u.y)]
     rw [mul_comm, ← Int.neg_mul]
     nth_rw 2 [← Int.mul_one (-(segment_start seg).u.y)]
     rw [← mul_add, neg_mul, mul_comm, add_right_comm]
     rw [Int.add_sub_cancel, add_comm]; congr
-    rw [← Int.natCast_one, ← Int.natCast_add, Nat.sub_right_comm]
-    rw [← Nat.sub_add_comm hle₀]
-    rw [Int.natCast_sub hle₁]
-    rfl
+    rwa [← Int.natCast_one, ← Int.natCast_add, ks, Int.natCast_sub]
   · repeat rw [add_right_comm _ _ (segment_start seg).u.x]
     nth_rw 2 [← Int.one_mul (segment_start seg).u.x]
     rw [← add_mul, add_right_comm, add_neg_cancel_right, add_comm]; congr
-    rw [← Int.natCast_one, ← Int.natCast_add, Nat.sub_right_comm]
-    rw [← Nat.sub_add_comm hle₀]
-    rw [Int.natCast_sub hle₁]
-    rfl
+    rwa [← Int.natCast_one, ← Int.natCast_add, ks, Int.natCast_sub]
 
 def segment_length_lb_prop (seg : TraceSegment) : Prop :=
   manhattan (loc (segment_start seg)) (loc (segment_end seg)) ≤ segment_length seg
@@ -490,43 +425,26 @@ lemma segment_length_lb_case1 (seg : TraceSegment) (h : segment_length seg = 1) 
 -- the segment begins with a 'move forward'
 lemma segment_length_lb_case2 (seg : TraceSegment) (h : 1 < segment_length seg) :
   segment_starts_with_move_forward seg h →
-  segment_length_lb_prop (segment_split_second seg (seg.i + 1) (Nat.le_add_right _ _)
-    (Nat.add_one_le_of_lt (Nat.lt_of_sub_pos (Nat.pos_of_lt_add_left h)))) →
+  segment_length_lb_prop (segment_split_second seg 1 h) →
   segment_length_lb_prop seg := by
   unfold segment_length_lb_prop
-  intro hmf hllb
-  let k := seg.i + 1
-  have lek : seg.i ≤ k := Nat.le_add_right _ _
-  have kle : k ≤ seg.j :=
-    Nat.add_one_le_of_lt (Nat.lt_of_sub_pos (Nat.pos_of_lt_add_left h))
-  rw [segment_split_length seg k lek kle]
-  rw [segment_split_first_length]
-  rw [Nat.sub_add_comm (Nat.le_refl seg.i), Nat.sub_self, zero_add]
-  rw [add_right_comm, Nat.add_one_sub_one, add_comm]
-  let seg_first := segment_split_first seg k lek kle
-  let seg_second := segment_split_second seg k lek kle
-  apply le_trans (manhattan_tri _ _ _)
-  change manhattan _ (loc (segment_start seg_second)) + _ ≤ _
-  rw [← segment_split_first_start seg k lek kle]
-  rw [← segment_split_second_end seg k lek kle]
-  nth_rw 1 [← segment_split_overlap]
-  rw [add_comm]
-  convert Nat.add_le_add_right hllb 1
-  unfold segment_starts_with_move_forward check_for_move at hmf
-  rw [← segment_start_eq_getElem_zero, getElem_congr_idx (Nat.zero_add _)] at hmf
-  rw [← segment_split_first_start seg k lek kle] at hmf
-  have : segment_end seg_first = (segment_states seg)[1]'(by rwa [segment_states_length]) := by
-    rw [segment_end_eq_getElem, getElem_congr_coll (segment_split_first_states _ _ _ _)]
-    rw [List.getElem_take]; congr
-    rw [segment_split_first_length, Nat.add_one_sub_one]
-    unfold k
-    rw [add_comm, Nat.add_sub_cancel]
-  rw [← this] at hmf
-  rw [← hmf]
-  let s := segment_start seg_first
-  change manhattan (loc s) (loc (move_forward s)) = 1
-  unfold manhattan move_forward loc; simp
-  exact uvec_xabs_add_yabs_eq_one _
+  let seg_first := segment_split_first seg 1 h
+  let seg_second := segment_split_second seg 1 h
+  intro hmf hman₁
+  have ltsl : 1 < (segment_states seg).length := by rwa [segment_states_length]
+  have hman₀ : manhattan (loc (segment_start seg)) (loc ((segment_states seg)[1]'ltsl)) = 1 := by
+    unfold segment_starts_with_move_forward check_for_move at hmf
+    rw [getElem_congr_idx (Nat.zero_add 1)] at hmf
+    rw [← hmf, ← segment_start_eq_getElem_zero, manhattan]
+    unfold loc move_forward; simp
+    exact uvec_xabs_add_yabs_eq_one _
+  rw [← segment_split_overlap, segment_end_eq_getElem] at hman₁
+  rw [segment_split_first_states_getElem, segment_split_second_end] at hman₁
+  have idxrw := congrArg (fun n ↦ n - 1) (segment_split_first_length seg 1 h)
+  dsimp at idxrw
+  rw [getElem_congr_idx idxrw, segment_split_second_length] at hman₁
+  convert le_trans (manhattan_tri _ _ _) (Nat.add_le_add (le_of_eq hman₀) hman₁)
+  rw [add_comm, Nat.sub_one_add_one (Nat.ne_zero_of_lt h)]
 
 -- Prove the segment length lower bound for 'L segments
 lemma segment_length_lb_case3 (seg : TraceSegment) (h : 1 < segment_length seg) :
